code/hpke/Hacl.HPKE.Curve64_CP32_SHA256.fsti
@@ -7,11 +7,13 @@ module Hash = Spec.Agile.Hash
 
 noextract unfold
 let cs = (DH.DH_Curve25519, AEAD.CHACHA20_POLY1305, Hash.SHA2_256)
+noextract unfold
+let vale_p = Vale.X64.CPU_Features_s.(adx_enabled /\ bmi2_enabled)
 
-val setupBaseI: setupBaseI_st cs
+val setupBaseI: setupBaseI_st cs vale_p
 
-val setupBaseR: setupBaseR_st cs
+val setupBaseR: setupBaseR_st cs vale_p
 
-val sealBase: sealBase_st cs
+val sealBase: sealBase_st cs vale_p
 
-val openBase: openBase_st cs
+val openBase: openBase_st cs vale_p
