code/hpke/Hacl.HPKE.P256_CP256_SHA256.fsti
@@ -8,10 +8,10 @@ module Hash = Spec.Agile.Hash
 noextract unfold
 let cs = (DH.DH_P256, AEAD.CHACHA20_POLY1305, Hash.SHA2_256)
 
-val setupBaseI: setupBaseI_st cs
+val setupBaseI: setupBaseI_st cs True
 
-val setupBaseR: setupBaseR_st cs
+val setupBaseR: setupBaseR_st cs True
 
-val sealBase: sealBase_st cs
+val sealBase: sealBase_st cs True
 
-val openBase: openBase_st cs
+val openBase: openBase_st cs True
